theories/interop/wp_prims/write_foreign.v
@@ -35,7 +35,7 @@ Proof using.
 
   iApply wp_pre_cases_c_prim; [done..|].
   iExists (λ '(e', σ'),
-    e' = WrSE (ExprV #0) ∧
+    e' = WrSE (ExprO (OVal #0)) ∧
     σ' = CState (WrapstateC (χC ρc) (<[γ:=Bforeign (Mut, Some w')]> (ζC ρc)) (θC ρc) (rootsC ρc)) mem).
   iSplit. { iPureIntro; econstructor; eauto. }
   iIntros (? ? ? (? & ?)); simplify_eq.
